Update dependencies.

theories/heap.v
@@ -17,9 +17,9 @@ From hazel Require Import weakestpre notation ieff.
 Set Default Proof Using "Type".
 
 Class heapPreG Σ := HeapPreG {
-  heap_preG_iris :> invPreG Σ;
-  heap_preG_heap :> gen_heapPreG loc val Σ;
-  heap_preG_inv_heap :> inv_heapPreG loc val Σ;
+  heap_preG_iris :> invGpreS Σ;
+  heap_preG_heap :> gen_heapGpreS loc val Σ;
+  heap_preG_inv_heap :> inv_heapGpreS loc val Σ;
 }.
 
 Definition heapΣ : gFunctors :=
@@ -28,15 +28,17 @@ Instance subG_heapPreG {Σ} : subG heapΣ Σ → heapPreG Σ.
 Proof. solve_inG. Qed.
 
 Class heapG Σ := HeapG {
-  heapG_invG : invG Σ;
-  heapG_gen_heapG :> gen_heapG loc val Σ;
-  heapG_inv_heapG :> inv_heapG loc val Σ;
+  heapG_invG : invGS Σ;
+  heapG_gen_heapG :> gen_heapGS loc val Σ;
+  heapG_inv_heapG :> inv_heapGS loc val Σ;
 }.
 
-Global Instance heapG_irisG `{!heapG Σ} : irisG eff_lang Σ := {
-  iris_invG := heapG_invG;
-  state_interp σ _ _ := (gen_heap_interp σ.(heap))%I;
+Global Instance heapG_irisG `{!heapG Σ} : irisGS eff_lang Σ := {
+  iris_invGS := heapG_invG;
+  state_interp σ _ _ _ := (gen_heap_interp σ.(heap))%I;
   fork_post _ := True%I;
+  num_laters_per_step _ := 0;
+  state_interp_mono _ _ _ _ := fupd_intro _ _
 }.
 
 
@@ -66,8 +68,8 @@ Lemma ewp_alloc E Ψ v :
   ⊢ EWP ref v @ E <| Ψ |> {{ lk, ∃ (l : loc), ⌜ lk = #l ⌝ ∗ l ↦ v }}.
 Proof.
   rewrite ewp_unfold /ewp_pre //=.
-  iIntros (σ ??) "Hσ".
-  iMod (fupd_intro_mask' E ∅) as "Hclose". by apply empty_subseteq.
+  iIntros (σ ????) "Hσ".
+  iMod (fupd_mask_subseteq ∅) as "Hclose". by apply empty_subseteq.
   iModIntro. iSplitR.
   - iPureIntro. rewrite /reducible //=.
     set (l := fresh_locs (dom (gset loc) σ.(heap))).
@@ -75,11 +77,12 @@ Proof.
     apply (Ectx_prim_step _ _ _ _ EmptyCtx (ref v) (#l)); try done.
     by apply alloc_fresh.
   - iIntros (e₂ σ₂ Hstep).
+    destruct κ; [|done]. simpl in Hstep.
     destruct Hstep; destruct K  as [|Ki K]; [| destruct Ki; try naive_solver ].
     + simpl in H, H0. simplify_eq. inversion H1.
       iMod (gen_heap_alloc _ l v with "Hσ") as "($ & Hl & Hm)". { done. }
       iApply ewp_value. simpl. iExists l. iFrame.
-      iIntros "!> !>". iMod "Hclose". iModIntro. by iPureIntro.
+      iIntros "!> !> !>". iMod "Hclose". iModIntro. by iPureIntro.
     + destruct (fill_val' K e1' v) as [-> ->]. naive_solver. by inversion H1.
 Qed.
 
@@ -87,20 +90,21 @@ Lemma ewp_load E Ψ l q v :
   l ↦{q} v -∗ EWP (Load #l)%E @ E <| Ψ |> {{ v', ⌜ v' = v ⌝ ∗ l ↦{q} v }}.
 Proof.
   iIntros "Hl". rewrite ewp_unfold /ewp_pre //=.
-  iIntros (σ _ _) "Hσ".
+  iIntros (σ ????) "Hσ".
   iDestruct (gen_heap_valid (heap σ) l q v with "Hσ Hl") as "%".
   rename H into heap_valid.
-  iMod (fupd_intro_mask' E ∅) as "Hclose". by apply empty_subseteq.
+  iMod (fupd_mask_subseteq ∅) as "Hclose". by apply empty_subseteq.
   iModIntro. iSplitR.
   - iPureIntro. rewrite /reducible //=.
     exists [], (Val v), σ, []. simpl.
     apply (Ectx_prim_step _ _ _ _ EmptyCtx (Load #l) v); try done.
     by apply LoadS.
   - iIntros (e₂ σ₂ Hstep).
+    destruct κ; [|done]. simpl in Hstep.
     destruct Hstep; destruct K  as [|Ki K]; [| destruct Ki; try naive_solver ].
     + simpl in H, H0. simplify_eq. inversion H1. simplify_eq. iFrame.
       iApply ewp_value. simpl. iFrame.
-      iIntros "!> !>". iMod "Hclose". iModIntro. by iPureIntro.
+      iIntros "!> !> !>". iMod "Hclose". iModIntro. by iPureIntro.
     + destruct (fill_val' K e1' #l) as [-> ->]. naive_solver. by inversion H1.
 Qed.
 
@@ -108,17 +112,18 @@ Lemma ewp_store E Ψ l (v' v : val) :
   l ↦ v' -∗ EWP #l <- v @ E <| Ψ |> {{ _, l ↦ v }}.
 Proof.
   iIntros "Hl". rewrite ewp_unfold /ewp_pre //=.
-  iIntros (σ _ _) "Hσ".
+  iIntros (σ ????) "Hσ".
   iDestruct (gen_heap_valid with "Hσ Hl") as "%".
   rename H into heap_valid.
   iMod (gen_heap_update _ _ _ v with "Hσ Hl") as "[Hσ Hl]".
-  iMod (fupd_intro_mask' E ∅) as "Hclose". by apply empty_subseteq.
+  iMod (fupd_mask_subseteq ∅) as "Hclose". by apply empty_subseteq.
   iModIntro. iSplitR.
   - iPureIntro. rewrite /reducible //=.
     exists [], (#()), (state_upd_heap <[ l := v ]> σ), []. simpl.
     apply (Ectx_prim_step _ _ _ _ EmptyCtx (#l <- v) #()); try done.
     apply StoreS. by eauto.
   - iIntros (e₂ σ₂ Hstep).
+    destruct κ; [|done]. simpl in Hstep.
     destruct Hstep; destruct K  as [|Ki K]; [| destruct Ki; try naive_solver ].
     + simpl in H, H0. simplify_eq. inversion H1. simplify_eq. iFrame.
       iApply ewp_value. simpl. by iFrame.
